Switch to nat width for binary

Cpc/Logos.lean
@@ -251,7 +251,7 @@ inductive Term : Type where
   | Numeral : native_Int -> Term
   | Rational : native_Rat -> Term
   | String : native_String -> Term
-  | Binary : native_Int -> native_Int -> Term
+  | Binary : native_Nat -> native_Int -> Term
   | Type : Term
   | Stuck : Term
   | Apply : Term -> Term -> Term
@@ -349,10 +349,10 @@ def __eo_mk_apply : Term -> Term -> Term
 
 def __eo_empty_binary : Term := (Term.Binary 0 0)
 def __eo_binary_mod_w (w : native_Int) (n : native_Int) : Term :=
-  (Term.Binary w (native_mod_total n (native_int_pow2 w)))
+  (Term.Binary (native_int_to_nat w) (native_mod_total n (native_int_pow2 w)))
 
 def __eo_mk_binary (w : native_Int) (n : native_Int) : Term :=
-  (native_ite (native_zleq 0 w) (Term.Binary w (native_mod_total n (native_int_pow2 w))) Term.Stuck)
+  (native_ite (native_zleq 0 w) (Term.Binary (native_int_to_nat w) (native_mod_total n (native_int_pow2 w))) Term.Stuck)
 
 def __eo_is_ok : Term -> Term
   | x => (Term.Boolean (native_not (native_teq x Term.Stuck)))
